partial checkin after removing boundedindex dependency. must clean up

lib/Struct.v
@@ -1,121 +1,27 @@
-Require Import String Word List Arith.
-Require Import Lib.CommonTactics Lib.ilist Lib.StringBound Lib.StringEq.
+Require Import String Lib.Word List Arith.
 Require Import Equality Eqdep_dec FunctionalExtensionality.
+Require Import Lib.CommonTactics Lib.StringEq.
 
 Set Implicit Arguments.
 
-Lemma NoDup_app_comm:
-  forall {A} (l1 l2: list A), NoDup (l1 ++ l2) -> NoDup (l2 ++ l1).
-Proof.
-  induction l2; simpl; intros; [rewrite app_nil_r in H; auto|].
-  constructor.
-  - intro Hx. apply in_app_or, or_comm, in_or_app in Hx.
-    apply NoDup_remove_2 in H; elim H; auto.
-  - apply IHl2.
-    eapply NoDup_remove_1; eauto.
-Qed.
+Section Attribute.
+  Variable A: Type.
 
-Lemma NoDup_app_comm_ext:
-  forall {A} (l1 l2 l3 l4: list A),
-    NoDup (l1 ++ (l2 ++ l3) ++ l4) -> NoDup (l1 ++ (l3 ++ l2) ++ l4).
-Proof.
-  intros; apply NoDup_app_comm; apply NoDup_app_comm in H.
-  rewrite <-app_assoc with (n:= l1).
-  rewrite <-app_assoc with (n:= l1) in H.
-  apply NoDup_app_comm; apply NoDup_app_comm in H.
-  induction (l4 ++ l1).
-  - rewrite app_nil_l in *; apply NoDup_app_comm; auto.
-  - simpl in *; inv H; constructor; auto.
-    intro Hx; elim H2; clear H2.
-    apply in_app_or in Hx; destruct Hx.
-    + apply in_or_app; auto.
-    + apply in_app_or in H; destruct H.
-      * apply in_or_app; right; apply in_or_app; auto.
-      * apply in_or_app; right; apply in_or_app; auto.
-Qed.
-
-Lemma NoDup_app_1:
-  forall {A} (l1 l2: list A), NoDup (l1 ++ l2) -> NoDup l1.
-Proof.
-  induction l1; simpl; intros; auto.
-  inv H; constructor; eauto.
-  intro Hx; elim H2; apply in_or_app; auto.
-Qed.
-
-Lemma NoDup_app_2:
-  forall {A} (l1 l2: list A), NoDup (l1 ++ l2) -> NoDup l2.
-Proof.
-  induction l2; simpl; intros; auto.
-  constructor.
-  - apply NoDup_remove_2 in H.
-    intro Hx; elim H; apply in_or_app; auto.
-  - apply IHl2; eapply NoDup_remove_1; eauto.
-Qed.
-
-Section GenAttribute.
-  Variable Key: Type.
-  Variable ValueT: Key -> Type.
-
-  Record GenAttr :=
-    { genAttrKey : Key;
-      genAttrVal : ValueT genAttrKey }.
-
-  Variable Key_dec: forall k1 k2: Key, {k1 = k2} + {k1 <> k2}.
-
-  Definition MapGenAttrT := forall key, ValueT key.
-
-  Definition addKeyVal (m: MapGenAttrT) k (v: ValueT k) :=
-    fun k' =>
-      match Key_dec k k' with
-        | left Heq => match Heq with
-                        | eq_refl => v
-                      end
-        | right _ => m k'
-      end.
-
-  Definition disjUnionMap (domain1: list Key) (map1: MapGenAttrT) (domain2: list Key) (map2: MapGenAttrT) :=
-    fun k =>
-      match in_dec Key_dec k domain1 with
-        | left _ => map1 k
-        | right _ => map2 k
-      end.
-
-  Definition filtMap (m: MapGenAttrT) hide def :=
-    fun k =>
-      match in_dec Key_dec k hide with
-        | left _ => def k
-        | right _ => m k
-      end.
-
-End GenAttribute.
-
-Definition unionMap Key (ValueT: Key -> Type)
-                    (map1 map2: MapGenAttrT (fun k => option (ValueT k))) :=
-  fun k =>
-    match map1 k, map2 k with
-      | Some v, _ => Some v
-      | _, Some v => Some v
-      | _, _ => None
-    end.
-
-Section BoundedIndexFull.
-  Variable Kind: Type.
-
-  Record Attribute :=
-    { attrName : string;
-      attrType : Kind }.
+  Record Attribute := { attrName: string; attrType: A }.
 
   Lemma attribute_inv:
-    forall n1 n2 k1 k2,
-      {| attrName := n1; attrType := k1 |} = {| attrName := n2; attrType := k2 |} ->
+    forall n1 n2 k1 k2, {| attrName := n1; attrType := k1 |} = {| attrName := n2; attrType := k2 |} ->
       n1 = n2 /\ k1 = k2.
   Proof.
     intros; inv H; auto.
   Qed.
 
-  Definition Attribute_dec (kdec: forall (k1 k2: Kind), {k1 = k2} + {k1 <> k2})
+  Definition Attribute_dec (kdec: forall (k1 k2: A), {k1 = k2} + {k1 <> k2})
   : forall (a1 a2: Attribute), {a1 = a2} + {a1 <> a2}.
-  Proof. intros; repeat decide equality. Qed.
+  Proof.
+    intros;
+    repeat decide equality.
+  Qed.
 
   Fixpoint getAttribute (n: string) (attrs: list Attribute) :=
     match attrs with
@@ -124,6 +30,7 @@ Section BoundedIndexFull.
         if string_eq n (attrName attr) then Some attr
         else getAttribute n attrs'
     end.
+  
   
   Lemma in_NoDup_attr:
     forall a1 a2 attrs,
@@ -135,14 +42,43 @@ Section BoundedIndexFull.
     destruct H1; [subst|].
     - destruct H2; [auto|].
       inv H; elim H3.
-      replace an2 with (attrName {| attrName:= an2; attrType:= ab2 |}) by reflexivity.
+      replace an2 with (attrName {| attrName := an2; attrType := ab2 |}) by reflexivity.
       apply in_map; auto.
     - destruct H2.
       + subst; inv H.
         elim H3.
-        replace an2 with (attrName {| attrName:= an2; attrType:= ab1 |}) by reflexivity.
+        replace an2 with (attrName {| attrName := an2; attrType := ab1 |}) by reflexivity.
         apply in_map; auto.
       + inv H; apply IHattrs; auto.
+  Qed.
+  
+  Fixpoint getAttrType (n: string) (attrs: list Attribute) :=
+    match attrs with
+      | nil => None
+      | attr :: attrs' =>
+        if string_eq n (attrName attr)
+        then Some (attrType attr)
+        else getAttrType n attrs'
+    end.
+
+  Lemma getAttrType_attrType_getAttribute n attrs:
+    getAttrType n attrs = match getAttribute n attrs with
+                            | None => None
+                            | Some a => Some (attrType a)
+                          end.
+  Proof.
+    induction attrs; simpl; auto.
+    destruct (string_eq n (attrName a)); auto.
+  Qed.
+  
+  Definition namesOf (attrs: list Attribute) := map attrName attrs.
+
+  Lemma namesOf_app:
+    forall (l1 l2: list Attribute),
+      namesOf (l1 ++ l2) = namesOf l1 ++ namesOf l2.
+  Proof.
+    unfold namesOf; simpl; intros.
+    rewrite map_app; reflexivity.
   Qed.
 
   Lemma getAttribute_app:
@@ -202,492 +138,14 @@ Section BoundedIndexFull.
       remember (string_eq _ _) as seq; destruct seq; [inv H1|].
       apply IHattrs; auto.
   Qed.
-
-  Fixpoint restrictAttrs (d: list string) (attrs: list Attribute) :=
-    match attrs with
-      | nil => nil
-      | attr :: attrs' =>
-        if in_dec string_dec (attrName attr) d
-        then attr :: (restrictAttrs d attrs')
-        else restrictAttrs d attrs'
-    end.
-
-  Fixpoint complementAttrs (d: list string) (attrs: list Attribute) :=
-    match attrs with
-      | nil => nil
-      | attr :: attrs' =>
-        if in_dec string_dec (attrName attr) d
-        then complementAttrs d attrs'
-        else attr :: (complementAttrs d attrs')
-    end.
-
-  Definition BoundedIndexFull attrs := BoundedIndex (map attrName attrs).
-
-  Definition GetAttr
-               {attrs: list Attribute}
-               (idx : BoundedIndexFull attrs) :=
-    nth_Bounded _ attrs idx.
-
-  Definition GetAttrType
-               {attrs: list Attribute}
-               (idx : BoundedIndexFull attrs) :=
-    attrType (GetAttr idx).
-
-  Lemma BoundedIndexFull_one_attr (a: Attribute):
-    forall i: BoundedIndexFull (a :: nil), GetAttrType i = attrType a.
-  Proof.
-    intros.
-    destruct i as [bind [ib bi]].
-    destruct ib.
-    - simpl in bi; inversion bi; subst; auto.
-    - simpl in bi; destruct ib; inversion bi.
-  Qed.
-
-End BoundedIndexFull.
-
-Definition namesOf {A} (attrs: list (Attribute A)) := map (@attrName _) attrs.
-Hint Unfold attrName attrType namesOf.
-
-Lemma namesOf_app:
-  forall {A} (l1 l2: list (Attribute A)),
-    namesOf (l1 ++ l2) = namesOf l1 ++ namesOf l2.
-Proof.
-  unfold namesOf; simpl; intros.
-  rewrite map_app; reflexivity.
-Qed.
-
-Section BoundedProp.
-  Definition boundedPropIdx (A: Type) (l: list A) (P: BoundedIndex l -> Prop)
-             (i: nat): Prop.
-  Proof.
-    remember (nth_error l i) as v.
-    destruct v.
-    exact (P {| indexb := Build_IndexBound _ _ (eq_sym Heqv) |}).
-    exact True.
-  Defined.
-
-  Inductive boundedPropStep
-            (A: Type) (l: list A) (P: BoundedIndex l -> Prop) : nat -> Prop :=
-  | boundedPropO: boundedPropIdx P O -> boundedPropStep P O
-  | boundedPropS n: boundedPropStep P n -> boundedPropIdx P (S n) ->
-                    boundedPropStep P (S n).
-
-  Definition boundedProp (A: Type) (l: list A) (P: BoundedIndex l -> Prop)
-    := boundedPropStep P (Datatypes.length l - 1).
-
-  Lemma boundedProp_forall (A: Type) (l: list A) (P: BoundedIndex l -> Prop):
-    boundedProp P <-> (forall (i: BoundedIndex l), P i).
-  Proof.
-    split; intros.
-
-    - unfold boundedProp in H.
-      destruct i as [bind [ib bi]].
-      pose proof (lt_nth _ _ bi).
-      induction (Datatypes.length l); [omega|].
-      simpl in *.
-      destruct (Compare_dec.lt_dec ib n) as [Hlt|Hnlt].
-      + destruct n; [omega|].
-        simpl in H; inversion H; subst; clear H.
-        simpl in IHn.
-        apply IHn; auto.
-        replace (n - 0) with n by omega; assumption.
-      + assert (ib = n) by omega; subst; clear H0 Hnlt IHn.
-        replace (n - 0) with n in H by omega.
-        destruct n.
-        * destruct l; inversion bi; subst.
-          simpl in H; inversion H; clear H.
-          unfold boundedPropIdx in H0; simpl in H0.
-          match goal with
-            | [H: P {| indexb := {| boundi := ?pf1 |} |} |-
-               P {| indexb := {| boundi := ?pf2 |} |} ] =>
-              replace pf2 with pf1 by apply UIP
-          end.
-          exact H0.
-        * inversion H; subst; clear H H1.
-          remember (S n) as n'; clear Heqn' n; rename n' into n.
-          unfold boundedPropIdx in H2.
-
-          generalize dependent n; generalize dependent l; induction l; intros;
-          [destruct n; simpl in bi; inversion bi|].
-          destruct n.
-
-          simpl in H2, bi; inversion bi; subst.
-          match goal with
-            | [H: P {| indexb := {| boundi := ?pf1 |} |} |-
-               P {| indexb := {| boundi := ?pf2 |} |} ] =>
-              replace pf2 with pf1 by apply UIP
-          end.
-          exact H2.
-
-          simpl in H2, bi.
-          pose (fun i: BoundedIndex l =>
-                  P {| indexb := {| boundi := (boundi i): nth_error (a :: l)
-                                                                    (S (ibound i))
-                                                          = Some (bindex i)
-                                 |} |}) as P'.
-          apply (IHl P'); auto.
-          
-    - unfold boundedProp.
-      induction (Datatypes.length l);
-        [simpl; constructor; unfold boundedPropIdx; destruct l; simpl; auto|].
-      simpl in *.
-      destruct n;
-        [simpl; constructor; unfold boundedPropIdx; destruct l; simpl; auto|].
-      simpl in *.
-      constructor; replace (n - 0) with n in IHn by omega; [assumption|].
-      unfold boundedPropIdx.
-
-      clear -H.
-      generalize dependent l.
-      induction n; intros.
-
-      + destruct l; simpl; auto.
-        destruct l; simpl; auto.
-
-      + destruct l; [simpl; auto|].
-        pose (fun i: BoundedIndex l =>
-                P {| indexb := {| boundi := (boundi i): nth_error (a::l) (S (ibound i))
-                                                        = Some (bindex i) |} |}) as P'.
-        assert (forall i, P' i) as H' by (intros; apply H).
-        apply (IHn l P' H').
-  Qed.
-
-End BoundedProp.
-
-Hint Unfold boundedPropIdx boundedProp.
-
-Section BoundedMap.
-  
-  Lemma boundedMap_equal:
-    forall A (l: list A) (V: BoundedIndex l -> Type)
-           (f g: forall (i: BoundedIndex l), V i),
-      f = g <-> (forall i, f i = g i).
-  Proof.
-    split; intros.
-    - subst; reflexivity.
-    - apply functional_extensionality_dep; auto.
-  Qed.
-
-  Lemma boundedMap_equal_separate:
-    forall A (l: list A) (V: BoundedIndex l -> Type)
-           (f g: forall (i: BoundedIndex l), V i),
-      f = g <-> boundedProp (fun i => f i = g i).
-  Proof.
-    split; intros.
-    - apply boundedProp_forall.
-      apply boundedMap_equal.
-      assumption.
-    - apply boundedMap_equal.
-      apply boundedProp_forall.
-      assumption.
-  Qed.    
-
-End BoundedMap.
-
-Section AddUnion.
-
-  Definition disjUnionBounded
-             (l: list string) {A: BoundedIndex l -> Type}
-             (f1: forall i: BoundedIndex l, option (A i))
-             (f2: forall i: BoundedIndex l, option (A i)) :=
-    fun i => match f1 i, f2 i with
-               | Some x, _ => Some x
-               | _, Some x => Some x
-               | _, _ => None
-             end.
-
-  Section DisjUnionBoundedProp.
-    Variable l: list string.
-    Context {A: BoundedIndex l -> Type}.
-
-    Theorem noneImpDisjUnionNone
-            (f1: forall i: BoundedIndex l, option (A i))
-            (f2: forall i: BoundedIndex l, option (A i))
-            (f1None: f1 = fun _ => None)
-            (f2None: f2 = fun _ => None):
-      disjUnionBounded f1 f2 = fun _ => None.
-    Proof.
-      unfold disjUnionBounded.
-      apply functional_extensionality_dep; intros.
-      assert (H: f1 x = None) by (rewrite f1None; intuition).
-      assert (H2: f2 x = None) by (rewrite f2None; intuition).
-      subst; intuition.
-    Qed.
-
-    Theorem noneUnionImpDisjUnionSame1
-            (f1: forall i: BoundedIndex l, option (A i))
-            (f2: forall i: BoundedIndex l, option (A i))
-            (f1None: f1 = fun _ => None):
-      disjUnionBounded f1 f2 = f2.
-    Proof.
-      unfold disjUnionBounded.
-      apply functional_extensionality_dep; intros.
-      assert (H: f1 x = None) by (rewrite f1None; intuition).
-      subst; destruct (f2 x); intuition.
-    Qed.
-
-    Theorem noneUnionImpDisjUnionSame2
-            (f1: forall i: BoundedIndex l, option (A i))
-            (f2: forall i: BoundedIndex l, option (A i))
-            (f2None: f2 = fun _ => None):
-      disjUnionBounded f1 f2 = f1.
-    Proof.
-      unfold disjUnionBounded.
-      apply functional_extensionality_dep; intros.
-      assert (H: f2 x = None) by (rewrite f2None; intuition).
-      subst; destruct (f1 x); intuition.
-    Qed.
-
-    Theorem disjUnionNoneImpNone
-            (f1: forall i: BoundedIndex l, option (A i))
-            (f2: forall i: BoundedIndex l, option (A i)):
-      forall x, disjUnionBounded f1 f2 x = None ->
-                f1 x = None /\ f2 x = None.
-    Proof.
-      intros.
-      unfold disjUnionBounded in *.
-      destruct (f1 x), (f2 x).
-      discriminate.
-      discriminate.
-      discriminate.
-      intuition.
-    Qed.
-
-    Theorem disjUnionImpNone
-            (f1: forall i: BoundedIndex l, option (A i))
-            (f2: forall i: BoundedIndex l, option (A i)):
-      disjUnionBounded f1 f2 = (fun _ => None) ->
-      f1 = (fun _ => None) /\ f2 = fun _ => None.
-    Proof.
-      intros.
-      unfold disjUnionBounded in *.
-      match goal with
-        | H: ?x=?y |- _ => remember x as m1; remember y as m2; rewrite Heqm2
-      end.
-      assert (base: forall x, m1 x = m2 x) by (intros; rewrite H; reflexivity).
-      rewrite Heqm1, Heqm2 in base.
-      assert (H1: f1 = fun _ => None) by
-          (apply functional_extensionality_dep;
-           intros;
-           specialize (base x);
-           destruct (f1 x); intuition).
-      assert (H2: f2 = fun _ => None).
-      (apply functional_extensionality_dep;
-       intros;
-       specialize (base x);
-       rewrite H1 in base;
-       destruct (f2 x); intuition).
-      intuition.
-    Qed.
-
-    Lemma disjUnionBounded_prop:
-      forall l (A: BoundedIndex l -> Type) lm rm i,
-        @disjUnionBounded l A lm rm i =
-        match lm i with
-          | Some v => Some v
-          | None => rm i
-        end.
-    Proof.
-      intros.
-      unfold disjUnionBounded.
-      subst.
-      destruct (lm i), (rm i); auto.
-    Qed.
-  
-  End DisjUnionBoundedProp.
-
-  Definition addBounded
-             (l: list string) {A: BoundedIndex l -> Type}
-             (i: BoundedIndex l)
-             (v: A i)
-             (f: forall i: BoundedIndex l, A i) :=
-    fun i' => match BoundedString_eq_dec i i' with
-                | left Heq =>
-                  match Heq with
-                    | eq_refl => v
-                  end
-                | right _ => f i'
-              end.
-
-  Section AddBoundedProp.
-    Variable l: list string.
-    Variable A: BoundedIndex l -> Type.
-
-    Theorem addBoundedNotNone
-            (i: BoundedIndex l)
-            (v: A i)
-            (f: forall i: BoundedIndex l, option (A i))
-            (contra: addBounded _ (Some v) f = fun _ => None):
-      False.
-    Proof.
-      unfold addBounded in contra.
-      match goal with
-        | H: ?x=?y |- _ => remember x as m1; remember y as m2
-      end.
-      assert (base: forall x, m1 x = m2 x) by (intros; rewrite contra; reflexivity).
-      rewrite Heqm1, Heqm2 in base.
-      specialize (base i).
-      destruct (BoundedString_eq_dec i i).
-      destruct e.
-      discriminate.
-      intuition.
-    Qed.
-
-    Lemma addBounded_prop1:
-      forall l (A: BoundedIndex l -> Type) m i i' (Hii: i = i') v,
-        @addBounded l A i v m i' = match Hii with eq_refl => v end.
-    Proof.
-      intros; subst.
-      unfold addBounded.
-      destruct (BoundedString_eq_dec i' i').
-      - rewrite (UIP_refl _ _ e); auto.
-      - elim n; auto.
-    Qed.
-    
-    Lemma addBounded_prop2:
-      forall l (A: BoundedIndex l -> Type) m i i' v' (Hii: i <> i'),
-        @addBounded l A i' v' m i = m i.
-    Proof.
-      intros.
-      unfold addBounded.
-      destruct (BoundedString_eq_dec i' i); auto.
-      elim Hii; auto.
-    Qed.
-
-  End AddBoundedProp.
-
-End AddUnion.
-  
-Ltac boundedApplyTac1 :=
-  unfold IndexBound_head, IndexBound_tail;
-  match goal with
-    | [ |- context [addBounded
-                      {| bindex := _; indexb := {| ibound := _;
-                                                   boundi := ?pf1 |} |}
-                      _ _
-                      {| bindex := _; indexb := {| ibound := _;
-                                                   boundi := ?pf2 |} |}] ] =>
-      first [rewrite (addBounded_prop1 _ _ eq_refl) |
-             replace pf2 with pf1 by apply UIP; rewrite (addBounded_prop1 _ _ eq_refl)]
-  end.
-
-Ltac boundedApplyTac2 :=
-  rewrite addBounded_prop2 by (let x := fresh "x" in intro x; inversion x).
-
-Ltac boundedApplyTac :=
-  repeat rewrite disjUnionBounded_prop;
-  repeat (first [boundedApplyTac1 | boundedApplyTac2 |
-                 progress destruct_eq | auto]).
-
-Ltac boundedApplyTac1_H H pf1 pf2 :=
-  first [rewrite (addBounded_prop1 _ _ eq_refl) in H |
-         replace pf2 with pf1 in H by apply UIP;
-           rewrite (addBounded_prop1 _ _ eq_refl) in H].
-
-Ltac boundedApplyTac2_H H :=
-  let x := fresh "x" in
-  rewrite addBounded_prop2 in H by (intro x; inversion x).
-
-Ltac boundedApplyTac_H :=
-  unfold IndexBound_head, IndexBound_tail in *;
-  repeat
-    match goal with
-      | [H: context [addBounded
-                       {| bindex := _; indexb := {| ibound := _;
-                                                    boundi := ?pf1 |} |}
-                       _ _
-                       {| bindex := _; indexb := {| ibound := _;
-                                                    boundi := ?pf2 |} |}]
-         |- _ ] => 
-        (repeat rewrite disjUnionBounded_prop in H;
-         repeat (first [boundedApplyTac1_H H pf1 pf2 | boundedApplyTac2_H H]))
-      | [H: Some _ = None |- _] => inversion H
-      | [H: Some _ = Some _ |- _] => inversion H; clear H; subst
-    end.
-
-Ltac boundedMapTac :=
-  apply boundedMap_equal_separate;
-  repeat autounfold with *; repeat constructor; repeat autounfold with *;
-  repeat split; simpl; try boundedApplyTac.
+End Attribute.
 
 Section MapAttr.
-  Variable Kind: Type.
-  Variable type: Kind -> Type.
+  Variable A B: Type.
+  Variable f: A -> B.
+  Definition changeAttr (a: Attribute A) := (attrName a, f (attrType a)).
 
-  Definition mapAttr a := {| attrName := attrName a;
-                             attrType := type (attrType a) |}.
-
-  Definition addFirstBoundedIndex A attrs (a: Attribute A) (idx: BoundedIndexFull attrs):
-    BoundedIndexFull (a :: attrs).
-  Proof.
-    apply {| indexb :=
-               {| boundi := (boundi idx): nth_error (map (@attrName _) (a :: attrs))
-                                                    (S (ibound idx)) = Some (bindex idx) |} |}.
-  Defined.
-  
-  Fixpoint getNewIdx1 attrs (idx: BoundedIndexFull (map mapAttr attrs)):
-    BoundedIndexFull attrs.
-  Proof.
-    destruct attrs.
-    apply (BoundedIndex_nil _ idx).
-    destruct idx as [s [i pf]].
-    destruct i.
-    apply ({| indexb := {|
-                         boundi := pf: nth_error (map (@attrName _) (a :: attrs)) 0 =
-                                       Some s |} |}).
-    apply (addFirstBoundedIndex a
-             (getNewIdx1 attrs {| indexb :=
-                                    {| boundi := pf: nth_error (map (@attrName _)
-                                                                    (map mapAttr attrs)) i =
-                                                     Some s |} |})).
-  Defined.
-
-  Fixpoint getNewIdx2 attrs (idx: BoundedIndexFull attrs):
-    BoundedIndexFull (map mapAttr attrs).
-  Proof.
-    destruct attrs.
-    apply (BoundedIndex_nil _ idx).
-    destruct idx as [s [i pf]].
-    destruct i.
-    apply ({| indexb :=
-                {| boundi := pf: nth_error (map (@attrName _) (map mapAttr (a :: attrs))) 0 =
-                                 Some s |} |}).
-    apply (addFirstBoundedIndex
-             (mapAttr a)
-             (getNewIdx2 attrs {| indexb :=
-                                    {| boundi := pf: nth_error (map (@attrName _) attrs) i =
-                                                     Some s |} |})).
-  Defined.
-
-  Fixpoint mapAttrEq1 attrs:
-    forall (idx: BoundedIndexFull (map mapAttr attrs))
-           (val: type (GetAttrType (getNewIdx1 attrs idx))),
-      GetAttrType idx.
-  Proof.
-    destruct attrs; intros.
-    apply (BoundedIndex_nil _ idx).
-    destruct idx as [s [i pf]].
-    destruct i.
-    assumption.
-    apply (mapAttrEq1 attrs {| indexb :=
-                                 {| boundi := pf: nth_error (map (@attrName _)
-                                                                 (map mapAttr attrs)) i = Some s
-                                 |} |} val).
-  Defined.
-
-  Fixpoint mapAttrEq2 attrs:
-    forall (idx: BoundedIndexFull attrs) (val: GetAttrType (getNewIdx2 idx)),
-      type (GetAttrType idx).
-  Proof.
-    destruct attrs; intros.
-    apply (BoundedIndex_nil _ idx).
-    destruct idx as [s [i pf]].
-    destruct i.
-    assumption.
-    apply (mapAttrEq2 attrs {| indexb :=
-                                 {| boundi := pf: nth_error (map (@attrName _) attrs) i = Some s
-                                 |} |} val).
-  Defined.
-
+  Definition mapAttr (ls: list (Attribute A)) := map changeAttr ls.
 End MapAttr.
 
+Hint Unfold attrName attrType namesOf changeAttr mapAttr.
