lib/ilist.v
@@ -1,6 +1,13 @@
+Generalizable All Variables.
 Set Implicit Arguments.
 
-Require Import List String Arith CommonTactics.
+Set Asymmetric Patterns.
+
+Require Import Coq.Lists.List
+        Coq.Strings.String
+        Coq.Arith.Arith Program.Equality.
+Require Export Lib.VectorFacts.
+Require Coq.Vectors.Vector.
 
 Section ilist.
 
@@ -10,234 +17,112 @@ Section ilist.
      by our ADT notations uses these to implement notation-friendly
      method lookups.  *)
 
+  Import Vectors.VectorDef.VectorNotations.
+
   Variable A : Type. (* The indexing type. *)
   Variable B : A -> Type. (* The type of indexed elements. *)
 
-  Inductive ilist : list A -> Type :=
-  | icons : forall a As, B a -> ilist As -> ilist (a :: As)
-  | inil : ilist nil.
+  Inductive ilist: forall n, Vector.t A n -> Type :=
+  | inil: ilist (Vector.nil A)
+  | icons t n (vs: Vector.t A n) (v: B t) (ils: ilist vs): ilist (t :: vs).
 
-  (* Get the car of an ilist. *)
-
-  Definition ilist_hd (As : list A) (il : ilist As) :
+  Definition ilist_hd {n} {As : Vector.t A n} (il : ilist As) :
     match As return ilist As -> Type with
       | a :: As' => fun il => B a
-      | nil => fun _ => unit
+      | [] => fun _ => unit
     end il :=
-    match il with
-      | icons a As b As' => b
-      | inil => tt
-    end.
+    match As return
+          forall (il : ilist As),
+            match As return ilist As -> Type with
+              | a :: As' => fun il => B a
+              | [] => fun _ => unit
+            end il with
+      | a :: As => fun il => match il in ilist (a :: As) return B a with
+                                          | icons t n' vs v ils => v
+                                          | inil => idProp
+                                        end
+      | [] => fun il => tt
+    end il.
+
+  Definition ilist_hd' {n} {As : Vector.t A (S n)} (il : ilist As) :
+    B (Vector.hd As)
+    := Vector.caseS (fun n As => ilist As -> B (Vector.hd As))
+                           (fun a As m => ilist_hd) As il.
 
   (* Get the cdr of an ilist. *)
-
-  Definition ilist_tl (As : list A) (il : ilist As) :
+  Definition ilist_tl {n} {As : Vector.t A n} (il : ilist As) :
     match As return ilist As -> Type with
       | a :: As' => fun il => ilist As'
-      | nil => fun _ => unit
+      | [] => fun _ => unit
     end il :=
-    match il with
-      | icons a As b As' => As'
-      | inil => tt
-    end.
-
-  (* Membership in an indexed list. *)
-
-  Inductive ilist_In {a : A} (b : B a)
-  : forall (As : list A) (il : ilist As), Prop :=
-  | In_hd : forall As' (il : ilist As'),
-              ilist_In b (icons b il)
-  | In_tl : forall a' (b' : B a') As' (il : ilist As'),
-              ilist_In b il ->
-              ilist_In b (icons b' il).
-
-  (* ilists can be built from standard lists of sigma types *)
-
-  Fixpoint siglist2ilist (sigList : list (sigT B))
-  : ilist (map (@projT1 _ B) sigList) :=
-    match sigList
-          return ilist (map (@projT1 _ B) sigList) with
-      | nil => inil
-      | (existT a b) :: sigList' => icons b (siglist2ilist sigList')
-    end.
-
-  (* and vice versa. *)
-
-  Fixpoint ilist2siglist {As : list A} (il : ilist As) : list (sigT B) :=
-    match il with
-      | inil => nil
-      | icons a As b il' => (existT B a b) :: (ilist2siglist il')
-    end.
-
-  (* ilist2siglist is the inverse of siglist2ilist *)
-  Lemma siglist2ilist_id
-  : forall (sigList : list (sigT B)),
-      ilist2siglist (siglist2ilist sigList) = sigList.
-  Proof.
-    induction sigList; simpl; auto.
-    destruct a; simpl; congruence.
-  Qed.
-
-  (* and vice-versa. *)
-
-  Fixpoint ilist2siglist_map
-          As (il : ilist As)
-  : map (@projT1 _ B) (ilist2siglist il) = As :=
-    match il as il' in ilist As' return
-          map (@projT1 _ B) (ilist2siglist il') = As' with
-      | inil => eq_refl
-      | icons a As' b il' => f_equal (fun b' => cons a b') (ilist2siglist_map il')
-    end.
-
-  Lemma ilist2sislist_map_cons
-  : forall a b As (il il' : ilist As),
-      match ilist2siglist_map il in (_ = y) return (ilist y -> Prop) with
-        | eq_refl =>
-          fun il' => siglist2ilist (ilist2siglist il) = il'
-      end il'
-      ->
-      match
-        f_equal (fun b' : list A => a :: b') (ilist2siglist_map il) in (_ = y)
-        return (ilist y -> Prop)
-      with
-        | eq_refl =>
-          fun il' : ilist (a :: map (projT1 (P:=B)) (ilist2siglist il)) =>
-            icons b (siglist2ilist (ilist2siglist il)) = il'
-      end (icons b il').
-  Proof.
-    intros until il; destruct (ilist2siglist_map il); congruence.
-  Qed.
-
-  Lemma ilist2siglist_id
-  : forall As (il : ilist As),
-      match (ilist2siglist_map il) in (_ = y) return
-            forall (il' : ilist y), Prop
-      with
-        | eq_refl => fun il' => siglist2ilist (ilist2siglist il) = il'
-      end il.
-  Proof.
-    induction il; simpl; auto.
-    apply ilist2sislist_map_cons; auto.
-  Qed.
-
-  (* Looking up the ith value, returning None for indices not in the list *)
-
-  (* A dependent option. *)
-  Inductive Dep_Option : option A -> Type :=
-    | Dep_Some : forall a, B a -> Dep_Option (Some a)
-    | Dep_None : Dep_Option None.
-
-  (* [Dep_Option_elim] projects out the [B a] value from
-     a dependent option indexed with [Some a], and returns
-     a unit value otherwise. *)
-  Definition Dep_Option_elimT (a_opt : option A) : Type :=
-    match a_opt with
-      | Some a => B a
-      | None => unit
-    end.
-  Definition Dep_Option_elim (a_opt : option A)
-            (b_opt : Dep_Option a_opt) :=
-    match b_opt in Dep_Option a_opt' return
-          Dep_Option_elimT a_opt' with
-      | Dep_Some a b => b
-      | Dep_None => tt
-    end.
-
-  Fixpoint ith_error
-          (As : list A)
-          (il : ilist As)
-          (n : nat)
-          {struct n}
-  : Dep_Option (nth_error As n) :=
-    match n as n' return
-          ilist As
-          -> Dep_Option (nth_error As n')
-    with
-      | 0 => match As as As' return
-                   ilist As'
-                   -> Dep_Option (nth_error As' 0) with
-               | nil => fun il => Dep_None
-               | cons a As' => fun il => Dep_Some (ilist_hd il)
-             end
-      | S n => match As as As' return
-                     ilist As'
-                     -> Dep_Option (nth_error As' (S n)) with
-                 | nil => fun il => Dep_None
-                 | cons a As' =>
-                   fun il =>
-                     ith_error (ilist_tl il) n
-             end
+    match As return
+          forall (il : ilist As),
+            match As return ilist As -> Type with
+              | Vector.cons a _ As' => fun il => ilist As'
+              | Vector.nil => fun _ => unit
+            end il with
+      | a :: As => fun il => match il in ilist (a :: As) return ilist As with
+                               | icons t n' vs v ils => ils
+                               | inil => idProp
+                             end
+      | [] => fun il => tt
     end il.
 
-  (* Looking up the ith value, returning a default value
-     for indices not in the list. *)
-  Fixpoint ith_default
-          (default_A : A)
-          (default_B : B default_A)
-          (As : list A)
-          (il : ilist As)
-          (n : nat)
-  {struct As} : B (nth n As default_A) :=
-    match As as As', n as n' return ilist As' -> B (nth n' As' default_A) with
-        | a :: As', 0    => @ilist_hd _
-        | a :: As', S n' => fun il => ith_default default_B (ilist_tl il) n'
-        | nil     , 0    => fun il => default_B
-        | nil     , S n' => fun il => default_B
-    end il.
+  Definition ilist_tl'
+             {n} {As : Vector.t A (S n)} (il : ilist As)
+    : ilist (Vector.tl As) :=
+    Vector.caseS (fun n As => ilist As -> ilist (Vector.tl As))
+                 (fun a As m => ilist_tl) As il.
 
-  Lemma ilist_invert (As : list A) (il : ilist As) :
+
+    
+  Fixpoint ith
+             {m : nat}
+             {As : Vector.t A m}
+             (il : ilist As)
+             (n : Fin.t m)
+  : B (Vector.nth As n) :=
+    match n in Fin.t m return
+          forall (As : Vector.t A m),
+            ilist As
+            -> B (Vector.nth As n) with
+      | Fin.F1 k =>
+        fun As =>
+          Vector.caseS (fun n As => ilist As
+                                    -> B (Vector.nth As (@Fin.F1 n)))
+                       (fun h n t => ilist_hd) As
+      | Fin.FS k n' =>
+        fun As =>
+          Vector_caseS' Fin.t
+                        (fun n As n' => ilist As
+                                        -> B (Vector.nth As (@Fin.FS n n')))
+                        (fun h n t m il => ith (ilist_tl il) m)
+                        As n'
+    end As il.
+
+
+  Lemma ilist_invert {n} (As : Vector.t A n) (il : ilist As) :
     match As as As' return ilist As' -> Prop with
       | a :: As' => fun il => exists b il', il = icons b il'
-      | nil => fun il => il = inil
+      | [] => fun il => il = inil
     end il.
   Proof.
-    destruct il; eauto.
+    destruct As; dependent destruction il; simpl; eauto.
+  Qed.
+
+  Lemma ilist_invert' {n} (As : Vector.t A n) (il : ilist As) :
+    match As as As' return ilist As' -> Type with
+      | a :: As' => fun il => sigT (fun b => sigT (fun il' => il = icons b il'))
+      | [] => fun il => il = inil
+    end il.
+  Proof.
+    destruct As; dependent destruction il; eauto.
   Qed.
 
   (* The [ith_induction] tactic is for working with lookups of bounded indices.
-     It first inducts on n, then destructs the index list [As] and eliminates
-     the contradictory cases, then finally destructs any indexed list in the
+     It first inducts on n, then destructs the index Vector.t [As] and eliminates
+     the contradictory cases, then finally destructs any indexed Vector.t in the
      context with Bounds of [As]. *)
-
-  Ltac icons_invert :=
-    repeat match goal with
-             | [il : ilist (_ :: _) |- _]
-               => let il' := fresh "il" in
-                  let b' := fresh "b" in
-                  let il'_eq := fresh "il_eq" in
-                  generalize (ilist_invert il);
-                    intros il'; destruct il' as [b' [il' il'_eq]]; subst
-           end.
-
-  Ltac ith_induction n As :=
-    induction n; simpl; intros;
-    (destruct As; simpl in *;
-                  [intros; elimtype False; eapply lt_n_0; eassumption
-                  | icons_invert ]).
-
-  Lemma ith_default_In :
-    forall (n : nat)
-           (As : list A)
-           (il : ilist As)
-           (default_A : A)
-           (default_B : B default_A),
-      n < List.length As ->
-      ilist_In (ith_default default_B il n) il.
-  Proof.
-    ith_induction n As; simpl; constructor; eauto with arith.
-  Qed.
-
-  Lemma ith_default_indep :
-    forall (n : nat)
-           (As : list A)
-           (il : ilist As)
-           (default_A : A)
-           (default_B default_B' : B default_A),
-      n < List.length As ->
-      ith_default default_B il n = ith_default default_B' il n.
-  Proof.
-    ith_induction n As; simpl; eauto with arith.
-  Qed.
 
 End ilist.
 
@@ -245,33 +130,15 @@ End ilist.
 Section ilist_map.
   Context {A} (B : A -> Type).
 
-  Fixpoint imap_list (f : forall a : A, B a) (As : list A) : ilist B As
+  Import Vectors.VectorDef.VectorNotations.
+
+  Fixpoint imap_list (f : forall a : A, B a) {n} (As : Vector.t A n) : ilist _ As
     := match As with
-         | nil => inil _
-         | x::xs => @icons _ B x _ (f x) (imap_list f xs)
+         | [] => inil _
+         | x :: xs => @icons _ B x _ _ (f x) (imap_list f xs)
        end.
 
-  Fixpoint map_ilist {C} (f : forall (a : A), B a -> C) {As} (Bs : ilist B As) : list C
-    := match Bs with
-         | inil => nil
-         | icons _ _ x xs => (f _ x)::map_ilist f xs
-       end.
 End ilist_map.
-
-Section of_list.
-  Context {T : Type}.
-
-  Definition ilist_of_list : forall ls : list T, ilist (fun _ => T) ls := imap_list (fun _ => T) (fun x => x).
-  Definition list_of_ilist {T'} {is} (ls : ilist (fun _ : T' => T) is) : list T
-    := map_ilist (B := fun _ => T) (fun _ x => x) ls.
-
-  Lemma list_of_ilist_of_list ls : list_of_ilist (ilist_of_list ls) = ls.
-  Proof.
-    unfold list_of_ilist, ilist_of_list.
-    induction ls; simpl in *; f_equal; assumption.
-  Qed.
-End of_list.
-
 
 Ltac icons_invert :=
   repeat match goal with
@@ -283,445 +150,202 @@ Ltac icons_invert :=
                   intros il'; destruct il' as [b' [il' il'_eq]]; subst
          end.
 
-Ltac ith_induction n As :=
-  induction n; simpl; intros;
-  (destruct As; simpl in *;
-                [intros; elimtype False; eapply lt_n_0; eassumption
-                | icons_invert ]).
-
 Section ilist_imap.
 
-  (* Mapping a function over an indexed list. *)
+  (* Mapping a function over an indexed Vector.t. *)
+
+  Import Vectors.VectorDef.VectorNotations.
 
   Variable A : Type. (* The indexing type. *)
   Variable B B' : A -> Type. (* The two types of indexed elements. *)
-  Variable f : forall a, B a -> B' a. (* The function to map over the list. *)
+  Variable f : forall a, B a -> B' a. (* The function to map over the Vector.t. *)
 
-  Fixpoint imap (As : list A)
-           (il : ilist B As)
-  : ilist B' As :=
-    match il in ilist _ As return ilist _ As with
-      | icons a As b il' => icons a (f b) (imap il')
-      | inil => inil B'
+  Fixpoint imap {n} (As : Vector.t A n)
+    : ilist _ As -> ilist _ As :=
+    match As return ilist _ As -> ilist _ As with
+    | [] => fun il => inil _
+    | a :: As' => fun il => icons _ (f (ilist_hd il)) (@imap _ As' (ilist_tl il))
     end.
 
   (* [imap] behaves as expected with the [ith_default] lookup
      function. *)
-  Lemma ith_default_imap :
-    forall (n : nat)
-           (As : list A)
-           (il : ilist _ As)
-           (default_A : A)
-           (default_B : B default_A),
-      f (ith_default default_A default_B il n) =
-      ith_default default_A (f default_B) (imap il) n.
-  Proof.
-    induction n; destruct As; simpl; eauto;
-    intros; icons_invert; simpl; auto.
-  Qed.
-
-  (* Mapping [f] over a dependent option. *)
-  Definition Dep_Option_Map
-             (a_opt : option A)
-             (b_opt : Dep_Option B a_opt) :
-    Dep_Option B' a_opt :=
-    match b_opt with
-      | Dep_Some a b' => Dep_Some B' a (f b')
-      | Dep_None => Dep_None B'
-    end.
-
-  (* Applying [f] to the value projected from a dependent option [b_opt]
-     is the same as mapping [f] over the [b_opt] and projecting.
-   *)
-  Lemma Dep_Option_Map_elim
-  : forall (a_opt : option A)
-           (b_opt : Dep_Option B a_opt),
-      Dep_Option_elim (Dep_Option_Map b_opt) =
-      match a_opt return
-            Dep_Option B a_opt -> Dep_Option_elimT B' a_opt with
-        | Some a => fun b => f (Dep_Option_elim b)
-        | None => fun _ => tt
-      end b_opt.
-  Proof.
-    unfold Dep_Option_elim, Dep_Option_Map; destruct b_opt; reflexivity.
-  Qed.
-
-  (* Concrete values for [a_opt] produce corrolaries of
-     [Dep_Option_Map_elim] with nicer statements. *)
-  Corollary Dep_Option_Map_elim_Some
-  : forall (a : A)
-           (b_opt : Dep_Option B (Some a)),
-      Dep_Option_elim (Dep_Option_Map b_opt) = f (Dep_Option_elim b_opt).
-  Proof.
-    intros; eapply Dep_Option_Map_elim; eauto.
-  Qed.
-
-  Corollary Dep_Option_Map_elim_None
-  : forall (b_opt : Dep_Option B None),
-      Dep_Option_elim (Dep_Option_Map b_opt) = tt.
-  Proof.
-    intros; eapply Dep_Option_Map_elim; eauto.
-  Qed.
-
-  (* [imap] behaves as expected with the [ith_error] lookup
-     function as well, albeit with a more dependently-typed statement. *)
-  Lemma ith_error_imap :
-    forall (n : nat)
-           (As : list A)
+  Lemma ith_imap :
+    forall {n}
+           (m : Fin.t n)
+           (As : Vector.t A n)
            (il : ilist _ As),
-      Dep_Option_Map (ith_error il n) =
-      ith_error (imap il) n.
+      f (ith il m) = ith (imap il) m.
   Proof.
-    induction n; destruct As; simpl; eauto;
-    intros; icons_invert; simpl; auto.
+    induction m; intro.
+    - eapply Vector.caseS with (v := As); intros; simpl in *; dependent destruction il; reflexivity.
+    - revert m IHm.
+      pattern n, As.
+      match goal with
+        |- ?P n As =>
+        simpl; eapply (@Vector.rectS _ P); intros
+      end.
+      inversion m.
+      eapply IHm.
   Qed.
 
 End ilist_imap.
 
-Section ilist_izip.
-
-  (* Merging two indexed lists together. *)
-
-  Variable A : Type. (* The indexing type. *)
-  Variable B B' D : A -> Type. (* The three types of indexed elements. *)
-  Variable f : forall a, B a -> B' a -> D a.
-
-  (* The function which merges the two sets of elements. *)
-  Fixpoint izip (As : list A)
-           (il : ilist B As) (il' : ilist B' As)
-  : ilist D As :=
-    match As return ilist B As -> ilist B' As -> ilist D As with
-      | a :: As' =>
-        fun il il' =>
-          icons a (f (ilist_hd il) (ilist_hd il'))
-                (izip (ilist_tl il) (ilist_tl il'))
-      | nil => fun il il' => inil D
-    end il il'.
-
-  (* [izip] behaves as expected with the [ith_default] lookup
-     function. *)
-  Lemma ith_default_izip :
-    forall (n : nat)
-           (As : list A)
-           (il : ilist B As)
-           (il' : ilist B' As)
-           (default_A : A)
-           (default_B : B default_A)
-           (default_B' : B' default_A),
-      ith_default _ (f default_B default_B') (izip il il') n =
-      f (ith_default _ default_B il n) (ith_default _ default_B' il' n).
-  Proof.
-    induction n; destruct As; simpl; eauto;
-    intros; icons_invert; simpl; auto.
-  Qed.
-
-  (* Merging two dependent options together. *)
-  Definition Dep_Option_Zip
-             (a_opt : option A)
-             (b_opt : Dep_Option B a_opt)
-             (b'_opt : Dep_Option B' a_opt):
-    Dep_Option D a_opt :=
-    match a_opt return
-          Dep_Option B a_opt -> Dep_Option B' a_opt ->
-          Dep_Option D a_opt with
-      | Some a =>
-        fun b b' =>
-          Dep_Some D a (f (Dep_Option_elim b) (Dep_Option_elim b'))
-      | None => fun _ _ => Dep_None D
-    end b_opt b'_opt.
-
-  (* Projecting the combination of two dependent sums [b_opt] and [b'_opt]
-     is the same as combining the projections of [b_opt] and [b'_opt]. *)
-  Lemma Dep_Option_Zip_elim
-  : forall (a_opt : option A)
-           (b_opt : Dep_Option B a_opt)
-           (b'_opt : Dep_Option B' a_opt),
-      Dep_Option_elim (Dep_Option_Zip b_opt b'_opt) =
-      match a_opt return
-            Dep_Option B a_opt
-            -> Dep_Option B' a_opt
-            -> Dep_Option_elimT D a_opt with
-        | Some a => fun b b' => f (Dep_Option_elim b) (Dep_Option_elim b')
-        | None => fun _ _ => tt
-      end b_opt b'_opt.
-  Proof.
-    unfold Dep_Option_elim, Dep_Option_Zip; destruct b_opt; reflexivity.
-  Qed.
-
-  (* Concrete values for [a_opt] produce corrolaries of
-     [Dep_Option_Zip_elim] with nicer statements. *)
-  Corollary Dep_Option_Zip_elim_Some
-  : forall (a : A)
-           (b_opt : Dep_Option B (Some a))
-           (b'_opt : Dep_Option B' (Some a)),
-      Dep_Option_elim (Dep_Option_Zip b_opt b'_opt) =
-      f (Dep_Option_elim b_opt) (Dep_Option_elim b'_opt).
-  Proof.
-    intros; eapply Dep_Option_Zip_elim; eauto.
-  Qed.
-
-  Corollary Dep_Option_Zip_elim_None
-  : forall (b_opt : Dep_Option B None)
-           (b'_opt : Dep_Option B' None),
-      Dep_Option_elim (Dep_Option_Zip b_opt b'_opt) = tt.
-  Proof.
-    intros; eapply Dep_Option_Zip_elim; eauto.
-  Qed.
-
-  (* [izip] behaves as expected with the [ith_error] lookup
-     function as well, albeit with a more dependently-typed statement. *)
-
-  Lemma ith_error_izip :
-    forall (n : nat)
-           (As : list A)
-           (il : ilist B As)
-           (il' : ilist B' As),
-      ith_error (izip il il') n =
-      Dep_Option_Zip (ith_error il n) (ith_error il' n).
-  Proof.
-    induction n; destruct As; simpl; eauto;
-    intros; icons_invert; simpl; auto.
-  Qed.
-
-End ilist_izip.
-
 Section ilist_replace.
 
-  (* Replacing an element of an indexed list. *)
-  Variable A : Type. (* The indexing type. *)
-  Variable B : A -> Type. (* The two types of indexed elements. *)
+  Import Vectors.VectorDef.VectorNotations.
 
-  Program Fixpoint replace_Index
-           {B : A -> Type}
-           (n : nat)
-           (As : list A)
-           (il : ilist B As)
-           (new_b : Dep_Option_elimT B (nth_error As n))
-           {struct As} : ilist B As :=
-    match n return
-            ilist B As
-            -> Dep_Option_elimT B (nth_error As n)
-            -> ilist B As with
-      | 0 => match As return
-                   ilist B As
-                   -> Dep_Option_elimT B (nth_error As 0)
-                   -> ilist B As with
-               | nil =>
-                 fun il _ => inil _
-               | cons a Bound' =>
-                 fun il new_b =>
-                   icons _ new_b (ilist_tl il)
-             end
-      | S n => match As return
-                     ilist B As
-                     -> Dep_Option_elimT B (nth_error As (S n))
-                     -> ilist B As with
-                 | nil => fun il _ => inil _
-                 | cons a Bound' =>
-                   fun il new_b =>
-                     icons _ (ilist_hd il)
-                           (@replace_Index B n Bound'
-                                           (ilist_tl il) new_b)
-               end
-    end il new_b.
+  (* Replacing an element of an indexed Vector.t. *)
+  Context {A : Type}. (* The indexing type. *)
+  Context {B : A -> Type}. (* The two types of indexed elements. *)
 
-  Lemma replace_Index_overflow
-  : forall
-      (n : nat)
-      (As : list A)
+  Fixpoint replace_Index
+             {m}
+             (As : Vector.t A m)
+             (il : ilist _ As)
+             (n : Fin.t m)
+             (new_b : B (Vector.nth As n))
+             {struct n}
+    : ilist _ As :=
+    match n in Fin.t m return
+          forall (As : Vector.t A m),
+            ilist _ As
+            -> B (Vector.nth As n)
+            -> ilist _ As with
+    | Fin.F1 k =>
+      fun As =>
+        Vector.caseS (fun n As => ilist _ As
+                                  -> B (Vector.nth As (@Fin.F1 n))
+                                  -> ilist _ As)
+                     (fun h n t il new_b => icons _ new_b (ilist_tl il) ) As
+    | Fin.FS k n' =>
+      fun As =>
+        Vector_caseS' Fin.t
+                     (fun n As n' =>
+                          ilist _ As
+                          -> B (Vector.nth As (@Fin.FS n n'))
+                          -> ilist _ As)
+                     (fun h n t m il new_b => icons _ (ilist_hd il)
+                                                    (@replace_Index _ _ (ilist_tl il) _ new_b))
+                     As n'
+    end As il new_b.
+
+  Lemma ith_replace_Index_neq {m}
+    : forall
+      (n n' : Fin.t m)
+      (As : Vector.t A m)
       (il : ilist _ As)
-      (new_b : Dep_Option_elimT B (nth_error As n)),
-      List.length As <= n
-      -> replace_Index n il new_b = il.
-  Proof.
-    induction n; simpl;
-    (destruct As; intros;
-     [generalize (ilist_invert il); intros; subst; reflexivity |
-      icons_invert; simpl in *]).
-    - destruct (le_Sn_0 _ H).
-    - f_equal; auto with arith.
-  Qed.
-
-  Definition Dep_Option_elim_P2
-             {B B' : A -> Type}
-             (P : forall a, B a -> B' a -> Prop)
-             (a_opt : option A)
-             (b_opt : Dep_Option B a_opt)
-             (b'_opt : Dep_Option B' a_opt)
-      := match a_opt return
-               Dep_Option_elimT B a_opt -> Dep_Option_elimT B' a_opt -> Prop with
-           | Some a => P a
-           | None => fun _ _ => True
-         end (Dep_Option_elim b_opt) (Dep_Option_elim b'_opt).
-
-  Lemma Dep_Option_P2_refl
-  : forall n As b,
-      @Dep_Option_elim_P2 B _ (fun a b b' => b = b')
-                     (nth_error As n) b b.
-  Proof.
-    intros n As; destruct (nth_error As n); simpl; auto.
-  Qed.
-
-  Lemma ith_replace_Index_neq
-  : forall
-      (n : nat)
-      (As : list A)
-      (il : ilist _ As)
-      (n' : nat)
-      (new_b : Dep_Option_elimT B (nth_error As n')),
+      (new_b : B (Vector.nth As n')),
       n <> n'
-      -> Dep_Option_elim_P2
-           (fun a b b' => b = b')
-           (ith_error (replace_Index n' il new_b) n)
-           (ith_error il n).
+      -> ith (replace_Index il n' new_b) n = ith il n.
   Proof.
-    unfold Dep_Option_elim_P2.
-    induction n; simpl; destruct As; intros; icons_invert;
-    simpl in *; auto;
-    destruct n'; simpl; try congruence.
-    eapply Dep_Option_P2_refl.
-    eapply IHn; congruence.
+    intros n n'; pattern m, n, n'.
+    match goal with
+      |- ?P m n n' => simpl; eapply (Fin.rect2 P); intros
+    end.
+    - congruence.
+    - generalize il f new_b; clear f new_b il H.
+      pattern n0, As.
+      match goal with
+        |- ?P n0 As =>
+        simpl; apply (@Vector.rectS _ P); intros; reflexivity
+      end.
+    - generalize il f new_b; clear f new_b il H.
+      pattern n0, As.
+      match goal with
+        |- ?P n0 As =>
+        simpl; apply (@Vector.rectS _ P); intros; reflexivity
+      end.
+    - assert (f <> g) by congruence.
+      generalize il f g new_b H H1; clear f g new_b il H H1 H0.
+      pattern n0, As.
+      match goal with
+        |- ?P n0 As =>
+        simpl; apply (@Vector.caseS _ P); intros;
+        dependent destruction il;
+        eapply (H _ il new_b); eauto
+      end.
   Qed.
 
-  Lemma ith_replace_Index_eq
-  : forall
-      (n : nat)
-      (As : list A)
+  Lemma ith_replace_Index_eq {m}
+    : forall
+      (n : Fin.t m)
+      (As : Vector.t A m)
       (il : ilist _ As)
-      (new_b : Dep_Option B (nth_error As n)),
-      Dep_Option_elim_P2
-        (fun a b b' => b = b')
-        (ith_error (replace_Index n il (Dep_Option_elim new_b)) n)
-        new_b.
+      (new_b : B (Vector.nth As n)),
+      ith (replace_Index il n new_b) n = new_b.
   Proof.
-    unfold Dep_Option_elim_P2.
-    induction n; destruct As; simpl; auto; intros; icons_invert.
-    apply IHn.
+    induction n; simpl.
+    - intro As; pattern n, As.
+      match goal with
+        |- ?P n As =>
+        simpl; apply (@Vector.caseS _ P); intros; reflexivity
+      end.
+    - intro As; revert n0 IHn; pattern n, As.
+      match goal with
+        |- ?P n As =>
+        simpl; apply (@Vector.caseS _ P); simpl; eauto
+      end.
   Qed.
 
 End ilist_replace.
 
-Section findIndex.
+Section ListToFunction.
+  Variable A: Type.
+  Variable B: A -> Type.
 
-  (* Find the index of an element in a list matching a comparator.
-     Originally used to look up the element of an ilist using ith_default. *)
+  Definition ilist_to_fun :=
+    fix ilist_to_fun n (vs : Vector.t A n) (ils : ilist (fun a : A => B a) vs)
+        {struct ils} :
+      forall i : Fin.t n, Vector.nth (Vector.map (fun p : A => B p) vs) i :=
+    match
+      vs in Vector.t _ k return (ilist (fun a : A => B a) vs ->
+                                 forall i : Fin.t k, Vector.nth (Vector.map (fun p : A => B p) vs) i)
+    with
+      | Vector.nil => fun _ i0 => Fin.case0 (Vector.nth (Vector.map (fun p : A => B p) (Vector.nil A))) i0
+      | Vector.cons a1 n1 vs1 =>
+        fun ils1 i1 =>
+          match ils1 in ilist _ (Vector.cons a n2 vs2) return
+                forall i2, Vector.nth (Vector.map (fun p: A => B p) (Vector.cons A a n2 vs2)) i2 with
+            | icons t3 n3 vs3 b ils3 =>
+              fun k =>
+                match k in Fin.t (S n4)
+                      return forall vs4 : Vector.t A n4,
+                               (forall i : Fin.t n4, Vector.nth (Vector.map (fun p : A => B p) vs4) i) ->
+                               Vector.nth (Vector.map (fun p : A => B p) (Vector.cons A t3 n4 vs4)) k with
+                  | Fin.F1 s5 => fun _ _ => b
+                  | Fin.FS s5 f5 => fun vs5 f => f f5
+                end vs3 (ilist_to_fun n3 vs3 ils3)
+          end i1
+    end ils.
+End ListToFunction.
 
-  Variable A : Type. (* The indexing type. *)
-  Variable C : Type. (* The type of comparators. *)
+Section ListToFunctionFun.
+  Variable A B: Type.
+  Variable f g: A -> Type.
+  Variable b_a: B -> A.
 
-  Variable AC_eq : A -> C -> bool. (* Comparision between index and comparator types. *)
-
-  Fixpoint findIndex (As : list A) (c : C)
-  : nat :=
-    match As with
-      | a :: As' => if AC_eq a c then 0 else S (findIndex As' c)
-      | _ => 0
-    end.
-
-  Lemma findIndex_In
-  : forall (As : list A) (c : C) (a : A),
-      In a As -> AC_eq a c = true ->
-      findIndex As c < List.length As.
-  Proof.
-    induction As; intros; simpl in *; intuition; subst.
-    - rewrite H0; auto with arith.
-    - find_if_inside; auto with arith.
-      generalize (@IHAs c _ H1 H0); auto with arith.
-  Qed.
-
-  Local Hint Resolve findIndex_In.
-
-  Lemma findIndex_NIn
-  : forall (As : list A) (c : C),
-      (forall a, In a As -> AC_eq a c = false) ->
-      findIndex As c = List.length As.
-  Proof.
-    induction As; intros; simpl in *; intuition; subst.
-    rewrite H; auto.
-  Qed.
-
-  Local Hint Resolve findIndex_NIn.
-
-  Lemma findIndex_In_dec
-  : forall (c : C) (As : list A),
-      (forall a, In a As -> AC_eq a c = false)
-      \/ (exists a, In a As /\ AC_eq a c = true).
-  Proof.
-    induction As; intros; simpl in *; intuition.
-    case_eq (AC_eq a c); intros; eauto.
-    left; intros; intuition; subst; eauto.
-    destruct_ex; intuition.
-    eauto.
-  Qed.
-
-  Lemma nth_findIndex_In
-  : forall (As : list A) (c : C) (a : A),
-      In a As -> AC_eq a c = true ->
-      forall a a',
-        nth (findIndex As c) As a = nth (findIndex As c) As a'.
-  Proof.
-    intros; apply nth_indep; eauto.
-  Qed.
-
-  Lemma AC_eq_nth_In
-  : forall (As : list A) (c : C) (a default_A : A),
-      In a As -> AC_eq a c = true ->
-      AC_eq (nth (findIndex As c) As default_A) c = true.
-  Proof.
-    induction As; simpl; intros; intuition;
-    case_eq (AC_eq a c); intros; eauto; subst; congruence.
-  Qed.
-
-  Lemma AC_eq_nth_NIn
-  : forall (As : list A) (c c' : C) (a default_A : A),
-      c <> c' ->
-      In a As -> AC_eq a c = true ->
-      (forall a, AC_eq a c = true -> AC_eq a c' = false) ->
-      AC_eq (nth (findIndex As c) As default_A) c' = false.
-  Proof.
-    induction As; simpl; intros; intuition;
-    case_eq (AC_eq a c); intros; eauto; subst; try congruence.
-  Qed.
-
-  Lemma nth_findIndex_NIn
-  : forall (As : list A) (c : C),
-      (forall a, In a As -> AC_eq a c = false) ->
-      forall a, nth (findIndex As c) As a = a.
-  Proof.
-    intros; apply nth_overflow; rewrite findIndex_NIn;
-    auto with arith.
-  Qed.
-
-  Lemma In_As
-        (As : list A)
-        (default_A : A)
-  : forall (a : A) (c : C),
-      List.In a As -> AC_eq a c = true ->
-      List.In (nth (findIndex As c) As default_A) As.
-  Proof.
-    induction As; simpl; intros; destruct H; subst.
-    - rewrite H0; auto.
-    - case_eq (AC_eq a c); intros; eauto.
-  Qed.
-
-  Lemma In_AC_eq
-        (AC_eq_c_c' :
-           forall a c c',
-             AC_eq a c = true
-             -> AC_eq a c' = true
-             -> c = c')
-        (As : list A)
-        (default_A : A)
-  : forall (a : A) (c c' : C),
-      List.In a As
-      -> AC_eq a c' = true
-      -> AC_eq (nth (findIndex As c') As default_A) c = true
-      -> c = c'.
-  Proof.
-    induction As; simpl; intros; destruct H; subst.
-    - case_eq (AC_eq a0 c'); intros; rewrite H in H1; eauto.
-      congruence.
-    - case_eq (AC_eq a c'); intros; rewrite H2 in H1; eauto.
-  Qed.
-
-End findIndex.
+  Definition ilist_to_fun_m (m: forall (k: A), f k -> g k) :=
+    (fix help n (vs : Vector.t (B) n) (ils : ilist (fun a => f (b_a a)) vs)
+         {struct ils} :
+       forall i : Fin.t n, Vector.nth (Vector.map (fun p => g (b_a p)) vs) i :=
+       match
+         vs in Vector.t _ k return (ilist (fun a => f (b_a a)) vs ->
+                                    forall i : Fin.t k, Vector.nth (Vector.map (fun p => g (b_a p)) vs) i)
+       with
+         | Vector.nil => fun _ i0 => Fin.case0 (Vector.nth (Vector.map (fun p => g (b_a p)) (Vector.nil _))) i0
+         | Vector.cons a1 n1 vs1 =>
+           fun ils1 i1 =>
+             match ils1 in ilist _ (Vector.cons a n2 vs2) return
+                   forall i2, Vector.nth (Vector.map (fun p => g (b_a p)) (Vector.cons _ a n2 vs2)) i2 with
+               | icons t3 n3 vs3 b ils3 =>
+                 fun k =>
+                   match k in Fin.t (S n4)
+                         return forall vs4 : Vector.t _ n4,
+                                  (forall i : Fin.t n4, Vector.nth (Vector.map (fun p => g (b_a p)) vs4) i) ->
+                                  Vector.nth (Vector.map (fun p => g (b_a p)) (Vector.cons _ t3 n4 vs4)) k with
+                     | Fin.F1 s5 => fun _ _ => (@m _ b)
+                     | Fin.FS s5 f5 => fun vs5 f => f f5
+                   end vs3 (help n3 vs3 ils3)
+             end i1
+       end ils).
+End ListToFunctionFun.
