lib/StringEq.v
@@ -1,6 +1,7 @@
 Require Import Bool Ascii String List.
 
 Set Implicit Arguments.
+Set Asymmetric Patterns.
 
 Definition ascii_eq (a1 a2: Ascii.ascii): bool :=
   match a1, a2 with
